Add identity type to term syntax

syntax.sig
@@ -10,3 +10,5 @@ tTrue : tm
 tFalse : tm
 tIf : tm -> tm -> tm -> tm
 tBool : tm
+tEq : tm -> tm -> tm -> tm
+tJ : (tm -> tm) -> tm -> tm -> tm -> tm
